WIP

Semantics/Dynamic/EvalRelation/Bool.v
@@ -8,11 +8,44 @@ From ExtensibleCompiler.Syntax.Terms Require Import
 
 From ExtensibleCompiler.Theory Require Import
      Functor
+     IndexedAlgebra
+     IndexedFunctor
+     IndexedProofAlgebra
+     IndexedSubFunctor
      SubFunctor
      UniversalProperty
 .
 
 Local Open Scope SubFunctor_scope.
+
+(* Class MyClass (T : Set) := {}. *)
+
+(* Class OtherClass (T : Set) `{MyClass T} := {}. *)
+
+(* Definition Pack (T : Set) := {t : T | True}. *)
+
+(* Axiom boolean : forall {T} `{OtherClass T}, bool -> Pack T. *)
+
+(* Section Bool. *)
+
+(*   Context {T} `{OtherClass T}. *)
+
+(*   Inductive EvalRelation__Bool *)
+(*             (EvalRelation__E : Pack T -> Prop) *)
+(*     : Pack T -> Prop *)
+(*     := *)
+(*     | BoolValue : forall b, EvalRelation__Bool EvalRelation__E (boolean b) *)
+(*   . *)
+
+(* End Bool. *)
+
+(* Derive Inversion inversion__Bool with *)
+(*     ( *)
+(*       forall {T} {CT : MyClass T} {OT : OtherClass T} *)
+(*         EvalRelation__E *)
+(*         e, *)
+(*         @EvalRelation__Bool T CT OT EvalRelation__E e *)
+(*     ). *)
 
 Section Bool.
 
@@ -33,7 +66,69 @@ Section Bool.
             (EvalRelation__E : (WellFormedValue E * WellFormedValue V) -> Prop)
     : (WellFormedValue E * WellFormedValue V) -> Prop
     :=
-    | BoolValue : forall b, EvalRelation__Bool EvalRelation__E (boolean b, boolean b)
+    | BoolValue : forall (b : bool), EvalRelation__Bool EvalRelation__E (boolean b, boolean b)
   .
+
+  Global Instance IndexedFunctor_EvalRelation__Bool
+    : IndexedFunctor (WellFormedValue E * WellFormedValue V) EvalRelation__Bool.
+  Proof.
+    constructor.
+    move => A B i IH [] b.
+    econstructor 1; apply IH => //.
+  Qed.
+
+  Variant ForEvalRelation := .
+
+  (**
+Sadly I can't find the incantation to make Coq generate this via [Derive
+Inversion], so manually written...
+   *)
+  Definition EvalInversion__Bool
+             (EvalRelation__E : WellFormedValue E * WellFormedValue V -> Prop)
+             (ev : WellFormedValue E * WellFormedValue V)
+             (P : (WellFormedValue E * WellFormedValue V)-indexedPropFunctor)
+             (IH : forall b : bool,
+                 P EvalRelation__E (boolean b, boolean b)
+             )
+             (ER : EvalRelation__Bool EvalRelation__E ev)
+    : P EvalRelation__E ev
+    :=
+      match ER in (EvalRelation__Bool _ p) return (p = ev -> P EvalRelation__E ev) with
+      | BoolValue _ b =>
+        fun EQ =>
+          eq_ind (boolean b, boolean b) (fun p => P EvalRelation__E p) (IH b) ev EQ
+      end eq_refl.
+
+  Definition EvalInversionClear__Bool
+             (EvalRelation__E : WellFormedValue E * WellFormedValue V -> Prop)
+             (ev : WellFormedValue E * WellFormedValue V)
+             (P : (WellFormedValue E * WellFormedValue V)-indexedPropFunctor)
+             (IH : forall b : bool,
+                 (boolean b, boolean b) = ev ->
+                 P EvalRelation__E (boolean b, boolean b))
+             (ER : EvalRelation__Bool EvalRelation__E ev)
+    : P EvalRelation__E ev
+    :=
+      match ER in (EvalRelation__Bool _ p) return (p = ev -> P EvalRelation__E ev) with
+      | BoolValue _ b =>
+        fun EQ =>
+          eq_ind (boolean b, boolean b) (fun p => P EvalRelation__E p) (IH b EQ) ev EQ
+      end eq_refl.
+
+  (* not sure if this is useful *)
+  Global Instance EvalRelationAlg__Bool
+         {A} `{FunctorLaws A}
+         `{SA : ! SubFunctor Bool A}
+         {EvalRelation__A : (WellFormedValue E * WellFormedValue V)-indexedPropFunctor}
+         `{! IndexedFunctor _ EvalRelation__A}
+         `{SE : ! IndexedSubFunctor EvalRelation__Bool EvalRelation__A}
+    : IndexedProofAlgebra ForEvalRelation EvalRelation__Bool (IndexedFix EvalRelation__A).
+  Proof.
+    constructor.
+    move => ev.
+    elim / @EvalInversionClear__Bool => b _.
+    apply (iInject (H1 := SE)).
+    apply BoolValue.
+  Qed.
 
 End Bool.
