Semantics/Dynamic/EvalRelation/If1.v
@@ -11,6 +11,7 @@ From ExtensibleCompiler.Syntax.Terms Require Import
 
 From ExtensibleCompiler.Theory Require Import
      Functor
+     IndexedFunctor
      SubFunctor
      UniversalProperty
 .
@@ -45,9 +46,43 @@ captures how [If1] evaluates in a larger language [E].
         EvalRelation__E (c, boolean true) ->
         EvalRelation__E (t, t') ->
         EvalRelation__If1 EvalRelation__E (if1 c t, t')
-    | If1alse : forall c t,
+    | If1False : forall c t,
         EvalRelation__E (c, boolean false) ->
         EvalRelation__If1 EvalRelation__E (if1 c t, unit)
   .
+
+  Global Instance IndexedFunctor_EvalRelation__If1
+    : IndexedFunctor (WellFormedValue E * WellFormedValue V) EvalRelation__If1.
+  Proof.
+    constructor.
+    move => A B i IH [].
+    - econstructor 1; apply IH => //.
+    - econstructor 2; apply IH => //.
+  Qed.
+
+  Definition EvalInversionClear__If1
+             (EvalRelation__E : WellFormedValue E * WellFormedValue V -> Prop)
+             (ev : WellFormedValue E * WellFormedValue V)
+             (P : (WellFormedValue E * WellFormedValue V)-indexedPropFunctor)
+             (IH__True : forall c t t',
+                 EvalRelation__E (c, boolean true) ->
+                 EvalRelation__E (t, t') ->
+                 (if1 c t, t') = ev ->
+                 P EvalRelation__E (if1 c t, t')
+             )
+             (IH__False : forall c t,
+                 EvalRelation__E (c, boolean false) ->
+                 (if1 c t, unit) = ev ->
+                 P EvalRelation__E (if1 c t, unit)
+             )
+             (ER : EvalRelation__If1 EvalRelation__E ev)
+    : P EvalRelation__E ev
+    :=
+      match ER in (EvalRelation__If1 _ p) return (p = ev -> P EvalRelation__E ev) with
+      | If1True _ c t t' E__c E__t =>
+        fun EQ => eq_ind (if1 c t, t') (P EvalRelation__E) (IH__True c t t' E__c E__t EQ) ev EQ
+      | If1False _ c t E__c =>
+        fun EQ => eq_ind (if1 c t, unit) (P EvalRelation__E) (IH__False c t E__c EQ) ev EQ
+      end eq_refl.
 
 End If1.
