Semantics/Dynamic/EvalRelation/If2.v
@@ -11,6 +11,7 @@ From ExtensibleCompiler.Syntax.Terms Require Import
 
 From ExtensibleCompiler.Theory Require Import
      Functor
+     IndexedFunctor
      SubFunctor
      UniversalProperty
 .
@@ -44,5 +45,40 @@ Section If2.
         EvalRelation__E (e, e') ->
         EvalRelation__If2 EvalRelation__E (if2 c t e, e')
   .
+
+  Global Instance IndexedFunctor_EvalRelation__If2
+    : IndexedFunctor (WellFormedValue E * WellFormedValue V) EvalRelation__If2.
+  Proof.
+    constructor.
+    move => A B i IH [].
+    - econstructor 1; apply IH => //.
+    - econstructor 2; apply IH => //.
+  Qed.
+
+  Definition EvalInversionClear__If2
+             (EvalRelation__E : WellFormedValue E * WellFormedValue V -> Prop)
+             (ev : WellFormedValue E * WellFormedValue V)
+             (P : (WellFormedValue E * WellFormedValue V)-indexedPropFunctor)
+             (IH__True : forall c t e t',
+                 EvalRelation__E (c, boolean true) ->
+                 EvalRelation__E (t, t') ->
+                 (if2 c t e, t') = ev ->
+                 P EvalRelation__E (if2 c t e, t')
+             )
+             (IH__False : forall c t e e',
+                 EvalRelation__E (c, boolean false) ->
+                 EvalRelation__E (e, e') ->
+                 (if2 c t e, e') = ev ->
+                 P EvalRelation__E (if2 c t e, e')
+             )
+             (ER : EvalRelation__If2 EvalRelation__E ev)
+    : P EvalRelation__E ev
+    :=
+      match ER in (EvalRelation__If2 _ p) return (p = ev -> P EvalRelation__E ev) with
+      | If2True _ c t e t' E__c E__t =>
+        fun EQ => eq_ind (if2 c t e, t') (P EvalRelation__E) (IH__True c t e t' E__c E__t EQ) ev EQ
+      | If2False _ c t e e' E__c E__e =>
+        fun EQ => eq_ind (if2 c t e, e') (P EvalRelation__E) (IH__False c t e e' E__c E__e EQ) ev EQ
+      end eq_refl.
 
 End If2.
