Semantics/Dynamic/Soundness/Unit.v
@@ -31,77 +31,77 @@ From ExtensibleCompiler.Theory Require Import
 
 Local Open Scope SubFunctor_scope.
 
-Section AbstractLemma.
+(* Section AbstractLemma. *)
 
-  Context
-    {T}
-    `{FunctorLaws T}
-    {C}
-    `{FunctorLaws C}
-    {E}
-    `{FunctorLaws E}
-    `{! E supports C}
-    `{! WellFormedSubFunctor C E}
-    {V}
-    `{FunctorLaws V}
-  .
+(*   Context *)
+(*     {T} *)
+(*     `{FunctorLaws T} *)
+(*     {C} *)
+(*     `{FunctorLaws C} *)
+(*     {E} *)
+(*     `{FunctorLaws E} *)
+(*     `{! E supports C} *)
+(*     `{! WellFormedSubFunctor C E} *)
+(*     {V} *)
+(*     `{FunctorLaws V} *)
+(*   . *)
 
-  Theorem EvenMoreAbstractSoundness
-         (WT__C : (TypedExpr T V)-indexedPropFunctor)
-         (WT__E : (TypedExpr T V)-indexedPropFunctor)
-         `(IndexedFunctor (TypedExpr T V) WT__C)
-         `(IndexedFunctor (TypedExpr T V) WT__E)
-         `(! IndexedSubFunctor WT__C WT__E)
+(*   Theorem EvenMoreAbstractSoundness *)
+(*          (WT__C : (TypedExpr T V)-indexedPropFunctor) *)
+(*          (WT__E : (TypedExpr T V)-indexedPropFunctor) *)
+(*          `(IndexedFunctor (TypedExpr T V) WT__C) *)
+(*          `(IndexedFunctor (TypedExpr T V) WT__E) *)
+(*          `(! IndexedSubFunctor WT__C WT__E) *)
 
-         `{Eval__C   : forall {R}, ProgramAlgebra ForEval   C R (EvalResult   V)}
-         `{Eval__E   : forall {R}, ProgramAlgebra ForEval   E R (EvalResult   V)}
-         `{! forall {R}, WellFormedProgramAlgebra Eval__C Eval__E (T := R)}
-         (recEval   : UniversalPropertyF E -> EvalResult   V)
+(*          `{Eval__C   : forall {R}, ProgramAlgebra ForEval   C R (EvalResult   V)} *)
+(*          `{Eval__E   : forall {R}, ProgramAlgebra ForEval   E R (EvalResult   V)} *)
+(*          `{! forall {R}, WellFormedProgramAlgebra Eval__C Eval__E (T := R)} *)
+(*          (recEval   : UniversalPropertyF E -> EvalResult   V) *)
 
-         `{TypeOf__C : forall {R}, ProgramAlgebra ForTypeOf C R (TypeOfResult T)}
-         `{TypeOf__E : forall {R}, ProgramAlgebra ForTypeOf E R (TypeOfResult T)}
-         `{! forall {R}, WellFormedProgramAlgebra TypeOf__C TypeOf__E (T := R)}
-         (recTypeOf : UniversalPropertyF E -> TypeOfResult T)
+(*          `{TypeOf__C : forall {R}, ProgramAlgebra ForTypeOf C R (TypeOfResult T)} *)
+(*          `{TypeOf__E : forall {R}, ProgramAlgebra ForTypeOf E R (TypeOfResult T)} *)
+(*          `{! forall {R}, WellFormedProgramAlgebra TypeOf__C TypeOf__E (T := R)} *)
+(*          (recTypeOf : UniversalPropertyF E -> TypeOfResult T) *)
 
-         Gamma (ctor : C (WellFormedValue E))
+(*          Gamma (ctor : C (WellFormedValue E)) *)
 
-    :
-      (forall
-          (Gamma' : Environment.Environment (ValueFix V))
-          (a : UniversalPropertyF E * UniversalPropertyF E),
-          (forall tau : TypeFix T,
-              programAlgebra' TypeOf__E recTypeOf (unwrapUP' (proj1_sig (snd a))) =
-              Some tau ->
-              WellTyped WT__E tau
-                        (programAlgebra' Eval__E recEval (unwrapUP' (proj1_sig (fst a)))
-                                         Gamma')) ->
-          forall tau : TypeFix T,
-            recTypeOf (snd a) = Some tau ->
-            WellTyped WT__E tau (recEval (wrapUP' (unwrapUP' (proj1_sig (fst a)))) Gamma')) ->
-      forall tau : TypeFix T,
-        programAlgebra' TypeOf__E recTypeOf (unwrapUP' (proj1_sig (inject ctor))) = Some tau ->
+(*     : *)
+(*       (forall *)
+(*           (Gamma' : Environment.Environment (ValueFix V)) *)
+(*           (a : UniversalPropertyF E * UniversalPropertyF E), *)
+(*           (forall tau : TypeFix T, *)
+(*               programAlgebra' TypeOf__E recTypeOf (unwrapUP' (proj1_sig (snd a))) = *)
+(*               Some tau -> *)
+(*               WellTyped WT__E tau *)
+(*                         (programAlgebra' Eval__E recEval (unwrapUP' (proj1_sig (fst a))) *)
+(*                                          Gamma')) -> *)
+(*           forall tau : TypeFix T, *)
+(*             recTypeOf (snd a) = Some tau -> *)
+(*             WellTyped WT__E tau (recEval (wrapUP' (unwrapUP' (proj1_sig (fst a)))) Gamma')) -> *)
+(*       forall tau : TypeFix T, *)
+(*         programAlgebra' TypeOf__E recTypeOf (unwrapUP' (proj1_sig (inject ctor))) = Some tau -> *)
 
-        (WT__C (IndexedFix WT__E) ({|
-             type := tau;
-             expr := programAlgebra' Eval__E recEval (unwrapUP' (proj1_sig (inject ctor))) Gamma;
-           |})) ->
+(*         (WT__C (IndexedFix WT__E) ({| *)
+(*              type := tau; *)
+(*              expr := programAlgebra' Eval__E recEval (unwrapUP' (proj1_sig (inject ctor))) Gamma; *)
+(*            |})) -> *)
 
 
-        WellTyped WT__E tau
-                  (programAlgebra' Eval__E recEval (unwrapUP' (proj1_sig (inject ctor))) Gamma).
-  Proof.
-    rewrite / inject /=.
-    rewrite unwrapUP'_wrapF /=.
-    rewrite fmapFusion / Extras.compose /=.
-    rewrite wellFormedSubFunctor => //=.
-    rewrite / programAlgebra'.
-    rewrite wellFormedProgramAlgebra.
-    rewrite wellFormedProgramAlgebra.
-    move => IH tau TY.
-    apply (iInject (F := WT__C)) => /=.
-  Qed.
+(*         WellTyped WT__E tau *)
+(*                   (programAlgebra' Eval__E recEval (unwrapUP' (proj1_sig (inject ctor))) Gamma). *)
+(*   Proof. *)
+(*     rewrite / inject /=. *)
+(*     rewrite unwrapUP'_wrapF /=. *)
+(*     rewrite fmapFusion / Extras.compose /=. *)
+(*     rewrite wellFormedSubFunctor => //=. *)
+(*     rewrite / programAlgebra'. *)
+(*     rewrite wellFormedProgramAlgebra. *)
+(*     rewrite wellFormedProgramAlgebra. *)
+(*     move => IH tau TY. *)
+(*     apply (iInject (F := WT__C)) => /=. *)
+(*   Qed. *)
 
-End AbstractLemma.
+(* End AbstractLemma. *)
 
 Section Unit.
 
