Theory/IndexedProofAlgebra.v
@@ -1,0 +1,86 @@
+From Coq Require Import
+     ssreflect
+.
+
+From ExtensibleCompiler.Theory Require Import
+     IndexedAlgebra
+     IndexedFunctor
+     IndexedSubFunctor
+     IndexedSum1
+     UniversalProperty
+.
+
+Local Open Scope SubFunctor_scope.
+Local Open Scope Sum1_scope.
+
+Class IndexedProofAlgebra (* cf. [iPAlgebra] *)
+      (Label : Set) {I} F `{IndexedFunctor I F} A :=
+  {
+    indexedProofAlgebra (* cf. [ip_algebra] *)
+    : IndexedAlgebra F A;
+  }.
+
+Definition indexedProofAlgebra'
+           {Label I F A}
+           `{IndexedFunctor I F}
+           (PA : IndexedProofAlgebra Label F A)
+  : IndexedAlgebra F A
+  := indexedProofAlgebra (IndexedProofAlgebra := PA).
+
+Global Instance
+       IndexedProofAlgebraSum1
+       {Label I} F G {A}
+       `{IndexedFunctor I F} `{IndexedFunctor I G}
+       {FAlg : IndexedProofAlgebra Label F A}
+       {GAlg : IndexedProofAlgebra Label G A}
+  : IndexedProofAlgebra Label (F + G) A
+  :=
+    {|
+      indexedProofAlgebra :=
+        fun i fg =>
+          match fg with
+          | iinl1 f => indexedProofAlgebra i f
+          | iinr1 g => indexedProofAlgebra i g
+          end
+      ;
+    |}.
+
+Set Typeclasses Debug.
+
+Class WellFormedIndexedProofAlgebra (* cf. [iWF_Ind] *)
+      {Label I F G}
+      `{IndexedFunctor I F} `{IndexedFunctor I G}
+      `{S : ! IndexedSubFunctor F G}
+      {P : forall i, IndexedFix G i -> Prop}
+      `(PA : ! IndexedProofAlgebra Label F (fun i => sig (P i)))
+  :=
+    {
+      indexedProjEq
+      : forall i e,
+        proj1_sig (indexedProofAlgebra (IndexedProofAlgebra := PA) i e)
+        =
+        iWrapF i (iInj (IndexedSubFunctor := S) (indexedFmap i (fun i => proj1_sig (P := P i)) e));
+    }.
+
+(** TODO: document why we need this *)
+Class WellFormedIndexedProofAlgebra2 (* cf. [WF_Ind2] *)
+      {Label I F G H}
+      `{IndexedFunctor I F} `{IndexedFunctor I G} `{IndexedFunctor I H}
+      `{SG : ! IndexedSubFunctor F G} `{SH : ! IndexedSubFunctor F H}
+      {P : forall i, (IndexedFix G i * IndexedFix H i) -> Prop}
+      `(PA : ! IndexedProofAlgebra Label F (fun i => sig (P i)))
+  :=
+    {
+      proj1Eq
+      : forall i e,
+        fst (proj1_sig (indexedProofAlgebra (IndexedProofAlgebra := PA) i e))
+        =
+        iWrapF i (iInj (IndexedSubFunctor := SG)
+                       (indexedFmap i (fun i e => fst (proj1_sig (P := P i) e)) e));
+      proj2Eq
+      : forall i e,
+        snd (proj1_sig (indexedProofAlgebra (IndexedProofAlgebra := PA) i e))
+        =
+        iWrapF i (iInj (IndexedSubFunctor := SH)
+                       (indexedFmap i (fun i e => snd (proj1_sig (P := P i) e)) e));
+    }.
